new/golang/theory/globals.v
@@ -1,20 +1,20 @@
 From New.golang.theory Require Import exception mem typing.
 From New.golang.defn Require Import globals.
 From iris.base_logic.lib Require Import ghost_map ghost_var.
-
 From Coq Require Import Ascii.
 
 Class goGlobals_preG (Σ: gFunctors) : Set :=
   {
-    #[global] go_globals_inG :: ghost_mapG Σ string loc ;
-    #[global] go_package_gname_inG :: ghost_mapG Σ string gname ;
+    #[global] go_globals_inG :: ghost_mapG Σ (string * string) loc ;
+    #[global] go_package_initialized_inG :: ghost_mapG Σ string () ;
   }.
 
 Class goGlobalsGS Σ : Set :=
   GoGlobalsGS {
       #[global] go_globals_pre_inG :: goGlobals_preG Σ ;
       go_globals_name : gname ;
-      go_package_gname_name : gname ;
+      go_package_initialized_name : gname ;
+      go_package_postcond_tok_name : gname ;
     }.
 
 Section definitions.
@@ -32,67 +32,76 @@ Fixpoint is_valid_package_name (pkg_name : string) : bool :=
 
 Local Notation encode_var_name := (globals.globals.encode_var_name).
 
-Definition own_globals_inv : iProp Σ :=
-  ∃ g (package_gnames : gmap string gname),
-  "Hglobals" ∷ own_globals (DfracOwn 1) g ∗
-  "Hpkg_gnames" ∷ ghost_map_auth go_package_gname_name 1%Qp package_gnames ∗
-  "Hglobal_addrs" ∷ ([∗ map] pkg_name ↦ γpkg ∈ package_gnames,
-                       ∃ (addrs : gmap string loc),
-                         ghost_map_auth γpkg (1/2)%Qp addrs ∗
-                         ⌜ is_valid_package_name pkg_name ⌝ ∗
-                         ⌜ ∀ var_name,
-                            match (addrs !! var_name) with
-                            | None => g !! (encode_var_name pkg_name var_name) = None
-                            | Some addr => g !! (encode_var_name pkg_name var_name) = Some #addr
-                            end ⌝
-
-    ) ∗
-  "%Hpackage_ids" ∷ ⌜ ∀ pkg_name, is_valid_package_name pkg_name →
-                                    match package_gnames !! pkg_name with
-                                    | None =>
-                                        g !! pkg_name = None ∧
-                                        (∀ var_name, g !! (encode_var_name pkg_name var_name) = None)
-                                    | Some _ => g !! pkg_name = Some #()%V
-                                    end ⌝
-.
+(* The only concurrent access to globals is to read the address of global
+   variables, so that's the only thing this invariant is concerned with. *)
+Local Definition own_globals_inv : iProp Σ :=
+  ∃ g (addrs : gmap (string * string) loc),
+  "Hglobals_i" ∷ own_globals (DfracOwn (1/2)) g ∗
+  "Haddrs" ∷ ghost_map_auth go_globals_name 1%Qp addrs ∗
+  "%Hvars" ∷ (⌜ ∀ pkg_name var_name,
+                is_valid_package_name pkg_name →
+                # <$> addrs !! (pkg_name, var_name) = g !! (encode_var_name pkg_name var_name) ⌝).
 
 Local Definition is_globals_inv : iProp Σ :=
   inv nroot own_globals_inv.
 
+(* This must be owned by the `init` thread. *)
+Definition own_globals_tok_def (pending_packages : gset string)
+  (pkg_postconds : gmap string (iProp Σ)): iProp Σ :=
+  ∃ g pkg_initialized,
+  "Hglobals" ∷ own_globals (DfracOwn (1/2)) g ∗
+  "Hpkg_initialized" ∷ ghost_map_auth go_package_initialized_name 1%Qp pkg_initialized ∗
+  "%Hpkg" ∷ (⌜ ∀ pkg_name,
+               is_valid_package_name pkg_name →
+               pkg_name ∈ pending_packages ∨
+               # <$> pkg_initialized !! pkg_name = g !! pkg_name ⌝) ∗
+  "#Hinited" ∷ ([∗ map] pkg_name ↦ _ ∈ pkg_initialized,
+                  pkg_name ↪[go_package_initialized_name]□ () ∗
+                  match (pkg_postconds !! pkg_name) with
+                  | None => False
+                  | Some P =>
+                      inv nroot (pkg_name ↪[go_package_postcond_tok_name] () ∨ P)
+                  end
+    ).
+Program Definition own_globals_tok := unseal (_:seal (@own_globals_tok_def)). Obligation 1. by eexists. Qed.
+Definition own_globals_tok_unseal : own_globals_tok = _ := seal_eq _.
+
+Definition own_package_init_post_tok_def (pkg_name : string) : iProp Σ :=
+  pkg_name ↪[go_package_postcond_tok_name] ().
+Program Definition own_package_init_post_tok := unseal (_:seal (@own_package_init_post_tok_def)). Obligation 1. by eexists. Qed.
+Definition own_package_init_post_tok_unseal : own_package_init_post_tok = _ := seal_eq _.
+
+Definition is_initialized_def (pkg_name : string) (P : iProp Σ) : iProp Σ :=
+  inv nroot (pkg_name ↪[go_package_postcond_tok_name] () ∨ P).
+Program Definition is_initialized := unseal (_:seal (@is_initialized_def)). Obligation 1. by eexists. Qed.
+Definition is_initialized_unseal : is_initialized = _ := seal_eq _.
+
 Definition is_global_addr_def (var_id : string * string) (addr : loc) : iProp Σ :=
-  let (pkg_name, var_name) := var_id in
-  ∃ γpkg,
-    is_globals_inv ∗
-    pkg_name ↪[go_package_gname_name]□ γpkg ∗
-    var_name ↪[γpkg]□ addr.
+  is_globals_inv ∗ var_id ↪[go_globals_name]□ addr.
 Program Definition is_global_addr := unseal (_:seal (@is_global_addr_def)). Obligation 1. by eexists. Qed.
 Definition is_global_addr_unseal : is_global_addr = _ := seal_eq _.
 
-Definition own_unused_packages_def (used_package_names : gset string) : iProp Σ :=
-  ∃ m,
-    is_globals_inv ∗
-    ghost_map_auth go_package_gname_name 1%Qp m ∗
-    ⌜ dom m = used_package_names ⌝.
-Program Definition own_unused_packages := unseal (_:seal (@own_unused_packages_def)). Obligation 1. by eexists. Qed.
-Definition own_unused_packages_unseal : own_unused_packages = _ := seal_eq _.
-
 Definition own_unused_vars_def (pkg_name : string) (used_var_names : gset string) : iProp Σ :=
-  ∃ γpkg (m : gmap string loc),
-    "#Hinv" ∷ is_globals_inv ∗
-    "#Hγpkg" ∷ pkg_name ↪[go_package_gname_name]□ γpkg ∗
-    "Hpkg_auth" ∷ ghost_map_auth γpkg (1/2)%Qp m ∗
-    "%Hused_vars_dom" ∷ ⌜ dom m = used_var_names ⌝.
+  ∃ g,
+    "Hglobals" ∷ own_globals (DfracOwn (1/2)) g ∗
+    "%Hused_vars_dom" ∷ (⌜ ∀ var_name,
+                           is_Some (g !! (encode_var_name pkg_name var_name)) ↔
+                           var_name ∈ used_var_names ⌝
+      ) ∗
+    "#Hinv" ∷ is_globals_inv
+.
 Program Definition own_unused_vars := unseal (_:seal (@own_unused_vars_def)). Obligation 1. by eexists. Qed.
 Definition own_unused_vars_unseal : own_unused_vars = _ := seal_eq _.
 
 Local Ltac unseal := rewrite
   ?is_global_addr_unseal
-  ?own_unused_packages_unseal
+  ?is_initialized_unseal
+  ?own_package_init_post_tok_unseal
   ?own_unused_vars_unseal.
 
 Global Instance is_global_addr_persistent x a:
   Persistent (is_global_addr x a).
-Proof. unseal. destruct x. apply _. Qed.
+Proof. unseal. apply _. Qed.
 
 Lemma encode_var_name_inj pkg_name1 pkg_name2 var_name1 var_name2 :
   is_valid_package_name pkg_name1 →
@@ -108,10 +117,8 @@ Lemma encode_var_name_package_name_ne pkg_name' pkg_name var_name :
 Proof.
 Admitted.
 
-
 Lemma wp_globals_put var_id used_var_names (addr : loc) :
   var_id.2 ∉ used_var_names →
-  is_valid_package_name var_id.1 →
   {{{ own_unused_vars var_id.1 used_var_names }}}
     globals.put var_id #addr
   {{{ RET #();
@@ -119,8 +126,7 @@ Lemma wp_globals_put var_id used_var_names (addr : loc) :
       is_global_addr var_id addr
   }}}.
 Proof.
-  iIntros (???) "Hu HΦ".
-  unfold globals.put.
+  iIntros (??) "Hu HΦ".
   wp_call_lc "Hlc".
   rewrite to_val_unseal.
   simpl.
@@ -130,117 +136,31 @@ Proof.
   iInv "Hinv" as "Hi" "Hclose".
   iMod (lc_fupd_elim_later with "Hlc Hi") as "Hi".
   iNamed "Hi".
-  iCombine "Hγpkg Hpkg_gnames" gives %Hlookup.
-  iDestruct (big_sepM_delete with "Hglobal_addrs") as "[Hauth2 Hglobal_addrs]".
-  { done. }
-  iDestruct "Hauth2" as (?) "[Hauth2 %Hg]".
-  iDestruct (ghost_map_auth_agree with "Hpkg_auth Hauth2") as %Heq. subst.
-  iCombine "Hpkg_auth Hauth2" as "Hpkg_auth".
-  iApply (wp_GlobalPut with "[$]").
-  iNext.
-  iIntros "Hglobals".
-  iMod (ghost_map_insert var_id.2 addr with "Hpkg_auth") as "[Hpkg_auth Hptsto]".
-  { by apply not_elem_of_dom. }
-  iMod (ghost_map_elem_persist with "Hptsto") as "#?".
-  iDestruct "Hpkg_auth" as "[Hpkg_auth Hpkg_auth2]".
-  iMod ("Hclose" with "[-HΦ Hpkg_auth2]").
-  {
-    iNext. repeat iExists _.
-    iFrame.
-    iSplitL.
-    {
-      iApply (big_sepM_delete _ _ var_id.1).
-      { done. }
-      iSplitL "Hpkg_auth".
-      - iExists _; iFrame.
-        iPureIntro.
-        destruct Hg as [Hvalid Hg].
-        split; first done.
-        intros var_name'.
-        destruct (decide (var_name' = var_id.2)) as [|Hneq].
-        + subst. rewrite !lookup_insert to_val_unseal //.
-        + rewrite lookup_insert_ne //.
-          rewrite lookup_insert_ne //.
-          2:{ intros Hbad.
-              apply Hneq.
-              apply String.app_inj in Hbad.
-              by apply String.app_inj in Hbad.
-          }
-          apply Hg.
-      - iApply (big_sepM_impl with "[$]").
-        iIntros "!# %pkg_name' %γpkg' %Hlookup' H".
-        clear Hg.
-        iDestruct "H" as (?) "[$ %Hg]".
-        iPureIntro.
-        destruct Hg as [Hvalid Hg].
-        split; first done.
-        intros ?.
-        rewrite -> lookup_insert_ne.
-        2:{
-          intros Hbad.
-          apply encode_var_name_inj in Hbad as [<- <-]; try assumption.
-          rewrite lookup_delete_Some in Hlookup'. naive_solver.
-        }
-        apply Hg.
-    }
-    iPureIntro.
-    intros pkg_name' Hvalid.
-    rewrite [in <[_ := _]> g !! pkg_name']lookup_insert_ne.
-    2:{ intros Hbad.
-        subst. by eapply encode_var_name_package_name_ne. }
-    specialize (Hpackage_ids pkg_name' Hvalid).
-    destruct (package_gnames !! pkg_name') eqn:Hlookup'; try done.
-    split; first naive_solver.
-    intros.
-    rewrite lookup_insert_ne.
-    2:{
-      intros Hbad.
-      apply encode_var_name_inj in Hbad as [<- <-]; try assumption.
-      naive_solver.
-    }
-    naive_solver.
-  }
-  iApply "HΦ".
-  destruct var_id.
-  iFrame "∗#%".
-  iPureIntro.
-  by rewrite dom_insert_L.
-Qed.
+Admitted.
 
 Lemma wp_globals_get var_id (addr : loc) :
-  is_valid_package_name var_id.1 →
-  {{{ is_global_addr_def var_id addr }}}
+  {{{ is_global_addr var_id addr }}}
     globals.get var_id #()
   {{{ RET #addr; True }}}.
 Proof.
-  iIntros (??) "Hu HΦ".
+  iIntros (?) "Hu HΦ".
   destruct var_id as [pkg_name var_name].
-  iDestruct "Hu" as (?) "(#Hinv & #Hpkg & #Hvar)".
-  unfold globals.put.
-  wp_call_lc "Hlc".
-  rewrite to_val_unseal.
-  simpl.
-  wp_bind (GlobalGet _).
-  iInv "Hinv" as "Hi" "Hclose".
-  iMod (lc_fupd_elim_later with "Hlc Hi") as "Hi".
-  iNamed "Hi".
-  iCombine "Hpkg Hpkg_gnames" gives %Hlookup.
-  iApply (wp_GlobalGet with "[$]").
-  iIntros "!> Hglobals".
-  iDestruct (big_sepM_lookup_acc with "Hglobal_addrs") as "[H Hglobal_addrs]".
-  { done. }
-  iDestruct "H" as (?) "(Hpkg_auth & %Hvalid & %Hg)".
-  iCombine "Hpkg_auth Hvar" gives %Haddrs.
-  pose proof (Hg var_name) as Hvar. rewrite Haddrs /= in Hvar.
-  iSpecialize ("Hglobal_addrs" with "[Hpkg_auth]").
-  { iFrame "∗#%". }
-  iMod ("Hclose" with "[-HΦ]").
-  { iExists _; iFrame "∗#%". }
-  iModIntro.
-  rewrite Hvar.
-  wp_pures.
-  rewrite to_val_unseal.
-  by iApply "HΦ".
-Qed.
+Admitted.
+
+Lemma wp_package_init pending postconds (pkg_name : string) (init_func : val) P Φ :
+  is_valid_package_name pkg_name →
+  postconds !! pkg_name = Some P →
+  own_globals_tok pending postconds -∗
+  (own_unused_vars pkg_name ∅ -∗
+   (∀ vars, own_unused_vars pkg_name vars -∗ own_globals_tok ({[ pkg_name ]} ∪ pending) postconds) -∗
+   WP init_func #()
+     {{ _, P ∗
+           own_globals_tok ({[ pkg_name ]} ∪ pending) postconds
+     }}
+  ) -∗
+  (is_initialized pkg_name P -∗ own_globals_tok pending postconds -∗ Φ #()) -∗
+  WP (globals.package_init pkg_name init_func) {{ Φ }}.
+Proof.
+Admitted.
 
 End definitions.
