new/proof/globals_test.v
@@ -1,58 +1,122 @@
 From New.proof Require Import grove_prelude.
 From New.code.github_com.mit_pdos.gokv Require globals_test.
 From Perennial.algebra Require Import map.
-From New.proof Require Import std.
 
 Section proof.
 
 Context `{!heapGS Σ}.
 Context `{!goGlobalsGS Σ}.
 
-Definition is_defined : iProp Σ :=
-  "HglobalB" ∷ ∃ globalB_addr, is_global_addr globals_test.globalB globalB_addr ∗
-  "HglobalA" ∷ ∃ globalA_addr, is_global_addr globals_test.globalA globalA_addr ∗
-  "HglobalY" ∷ ∃ globalY_addr, is_global_addr globals_test.globalY globalY_addr ∗
-  "HGlobalX" ∷ ∃ GlobalX_addr, is_global_addr globals_test.GlobalX GlobalX_addr
+Definition own_defined : iProp Σ :=
+  ∃ globalB_addr globalA_addr globalY_addr GlobalX_addr,
+    "#HglobalB_addr" ∷ is_global_addr globals_test.globalB globalB_addr ∗
+    "HglobalB" ∷ globalB_addr ↦ (default_val string) ∗
+    "#HglobalA_addr" ∷ is_global_addr globals_test.globalA globalA_addr ∗
+    "HglobalA" ∷ globalA_addr ↦ (default_val string) ∗
+    "#HglobalY_addry" ∷ is_global_addr globals_test.globalY globalY_addr ∗
+    "HglobalY" ∷ globalY_addr ↦ (default_val string) ∗
+    "#HGlobalX_addr" ∷ is_global_addr globals_test.GlobalX GlobalX_addr ∗
+    "HGlobalX" ∷ GlobalX_addr ↦ (default_val w64)
 .
 
 Lemma wp_define' :
   {{{ own_unused_vars globals_test.pkg_name' ∅ }}}
     globals_test.define' #()
-  {{{ RET #(); is_defined }}}.
+  {{{ vars, RET #();
+      own_defined ∗
+      own_unused_vars globals_test.pkg_name' vars
+  }}}.
 Proof.
   iIntros (?) "Hunused HΦ".
   wp_call.
   rewrite -!default_val_eq_zero_val /=.
 
   wp_alloc globalB_ptr as "?".
-  wp_apply (wp_globals_put with "[Hunused]"); [| | iFrame |]; [set_solver | reflexivity |].
+  wp_apply (wp_globals_put with "[Hunused]"); [| iFrame |]; [set_solver | ].
   iIntros "[Hunused #?]".
   wp_pures.
 
   wp_alloc globalA_ptr as "?".
-  wp_apply (wp_globals_put with "[Hunused]"); [| | iFrame |]; [set_solver| reflexivity |].
+  wp_apply (wp_globals_put with "[Hunused]"); [| iFrame |]; [set_solver | ].
   iIntros "[Hunused #?]".
   wp_pures.
 
   wp_alloc globalY_ptr as "?".
-  wp_apply (wp_globals_put with "[Hunused]"); [| | iFrame |]; [set_solver| reflexivity |].
+  wp_apply (wp_globals_put with "[Hunused]"); [| iFrame |]; [set_solver | ].
   iIntros "[Hunused #?]".
   wp_pures.
 
   wp_alloc GlobalX_ptr as "?".
-  wp_apply (wp_globals_put with "[Hunused]"); [| | iFrame |]; [set_solver| reflexivity |].
+  wp_apply (wp_globals_put with "[Hunused]"); [| iFrame |]; [set_solver | ].
   iIntros "[Hunused #?]".
   wp_pures.
 
   iApply "HΦ".
-  iFrame "#".
+  iFrame "#∗".
 Qed.
 
+Definition own_initialized : iProp Σ :=
+  ∃ globalB_addr globalA_addr globalY_addr GlobalX_addr,
+  "#HglobalB_addr" ∷ is_global_addr globals_test.globalB globalB_addr ∗
+  "#HglobalA_addr" ∷ is_global_addr globals_test.globalA globalA_addr ∗
+  "#HglobalY_addr" ∷ is_global_addr globals_test.globalY globalY_addr ∗
+  "#HGlobalX_addr" ∷ is_global_addr globals_test.GlobalX GlobalX_addr ∗
+
+  "HglobalB" ∷ globalB_addr ↦ "b" ∗
+  "HglobalA" ∷ globalA_addr ↦ "a" ∗
+  "HglobalY" ∷ globalY_addr ↦ "" ∗
+  "HglobalX" ∷ GlobalX_addr ↦ (W64 10)
+.
+
+(* Pick an iProp that is given when initialized.
+ *)
+
 Lemma wp_initialize' :
-  {{{ True }}}
+  {{{ own_globals_tok ∅ {[ globals_test.pkg_name' := own_initialized ]} }}}
     globals_test.initialize' #()
-  {{{ RET #(); True }}}.
+  {{{ RET #(); own_initialized }}}.
 Proof.
+  iIntros (?) "Hunused HΦ".
+  wp_call.
+  wp_apply (wp_package_init with "[$]").
+  { reflexivity. }
+  { reflexivity. }
+  { (* prove init function *)
+    iIntros "Hvars Htok".
+    wp_pures.
+    wp_apply (wp_define' with "[$]").
+    iIntros (?) "[Hdefined Hvars]".
+    iSpecialize ("Htok" with "[$]").
+    iNamed "Hdefined".
+    wp_pures.
+
+    (* go into foo() *)
+    wp_call.
+    wp_apply (wp_globals_get with "[]"); first iFrame "#".
+    wp_store.
+    wp_pures.
+    wp_apply (wp_globals_get with "[]"); first iFrame "#".
+    wp_store.
+    wp_pures.
+    wp_apply (wp_globals_get with "[]"); first iFrame "#".
+    wp_store.
+    wp_pures.
+    wp_apply (wp_globals_get with "[]"); first iFrame "#".
+    wp_load.
+    wp_pures.
+    wp_apply (wp_globals_get with "[]"); first iFrame "#".
+    wp_store.
+    wp_pures.
+    wp_apply (wp_globals_get with "[]"); first iFrame "#".
+    wp_store.
+    wp_pures.
+    iFrame "Htok".
+    iFrame "∗#".
+  }
+  iIntros "His Htok".
+  iApply "HΦ".
+  iFrame.
+  (* FIXME: get token to claim postcond *)
 Admitted.
 
 End proof.
